ovn/tests/ovn_example.rs
@@ -36,90 +36,90 @@ pub use hacspec_ovn::*;
 // pub use ovn_group::*;
 // pub use ovn_trait::*;
 
-#[derive(Clone, Copy)]
-pub struct z_89 {}
-impl Z_Field for z_89 {
-    type field_type = u32;
-    fn q() -> Self::field_type {
-        89u32
-    } // Prime order
-    fn random_field_elem(random: u32) -> Self::field_type {
-        random % (Self::q() - 1)
-    }
+// #[derive(Clone, Copy)]
+// pub struct z_89 {}
+// impl Z_Field for z_89 {
+//     type field_type = u32;
+//     fn q() -> Self::field_type {
+//         89u32
+//     } // Prime order
+//     fn random_field_elem(random: u32) -> Self::field_type {
+//         random % (Self::q() - 1)
+//     }
 
-    fn field_zero() -> Self::field_type {
-        0u32
-    }
+//     fn field_zero() -> Self::field_type {
+//         0u32
+//     }
 
-    fn field_one() -> Self::field_type {
-        1u32
-    }
+//     fn field_one() -> Self::field_type {
+//         1u32
+//     }
 
-    fn add(x: Self::field_type, y: Self::field_type) -> Self::field_type {
-        (x + y) % (Self::q() - 1)
-    }
+//     fn add(x: Self::field_type, y: Self::field_type) -> Self::field_type {
+//         (x + y) % (Self::q() - 1)
+//     }
 
-    fn sub(x: Self::field_type, y: Self::field_type) -> Self::field_type {
-        (x + (Self::q() - 1) - y) % (Self::q() - 1)
-    }
+//     fn sub(x: Self::field_type, y: Self::field_type) -> Self::field_type {
+//         (x + (Self::q() - 1) - y) % (Self::q() - 1)
+//     }
 
-    fn mul(x: Self::field_type, y: Self::field_type) -> Self::field_type {
-        (x * y) % (Self::q() - 1)
-    }
-}
+//     fn mul(x: Self::field_type, y: Self::field_type) -> Self::field_type {
+//         (x * y) % (Self::q() - 1)
+//     }
+// }
 
-#[derive(Clone, Copy)]
-pub struct g_z_89 {}
-impl Group<z_89> for g_z_89 {
-    type group_type = u32;
+// #[derive(Clone, Copy)]
+// pub struct g_z_89 {}
+// impl Group<z_89> for g_z_89 {
+//     type group_type = u32;
 
-    fn g() -> Self::group_type {
-        3u32
-    } // Generator (elemnent of group)
+//     fn g() -> Self::group_type {
+//         3u32
+//     } // Generator (elemnent of group)
 
-    fn hash(x: Vec<Self::group_type>) -> <z_89 as Z_Field>::field_type {
-        let mut res = z_89::field_one();
-        for y in x {
-            res = z_89::mul(y, res);
-        }
-        res // TODO
-    }
+//     fn hash(x: Vec<Self::group_type>) -> <z_89 as Z_Field>::field_type {
+//         let mut res = z_89::field_one();
+//         for y in x {
+//             res = z_89::mul(y, res);
+//         }
+//         res // TODO
+//     }
 
-    fn g_pow(x: <z_89 as Z_Field>::field_type) -> Self::group_type {
-        Self::pow(Self::g(), x)
-    }
+//     fn g_pow(x: <z_89 as Z_Field>::field_type) -> Self::group_type {
+//         Self::pow(Self::g(), x)
+//     }
 
-    // TODO: use repeated squaring instead!
-    fn pow(g: Self::group_type, x: <z_89 as Z_Field>::field_type) -> Self::group_type {
-        let mut result = Self::group_one();
-        for i in 0..(x % (z_89::q() - 1)) {
-            result = Self::prod(result, g);
-        }
-        result
-    }
+//     // TODO: use repeated squaring instead!
+//     fn pow(g: Self::group_type, x: <z_89 as Z_Field>::field_type) -> Self::group_type {
+//         let mut result = Self::group_one();
+//         for i in 0..(x % (z_89::q() - 1)) {
+//             result = Self::prod(result, g);
+//         }
+//         result
+//     }
 
-    fn group_one() -> Self::group_type {
-        1
-    }
+//     fn group_one() -> Self::group_type {
+//         1
+//     }
 
-    fn prod(x: Self::group_type, y: Self::group_type) -> Self::group_type {
-        ((x % z_89::q()) * (y % z_89::q())) % z_89::q()
-    }
+//     fn prod(x: Self::group_type, y: Self::group_type) -> Self::group_type {
+//         ((x % z_89::q()) * (y % z_89::q())) % z_89::q()
+//     }
 
-    fn inv(x: Self::group_type) -> Self::group_type {
-        for j in 0..89 {
-            if Self::prod(x, j) == Self::group_one() {
-                return j;
-            }
-        }
-        assert!(false);
-        return x;
-    }
+//     fn inv(x: Self::group_type) -> Self::group_type {
+//         for j in 0..89 {
+//             if Self::prod(x, j) == Self::group_one() {
+//                 return j;
+//             }
+//         }
+//         assert!(false);
+//         return x;
+//     }
 
-    fn div(x: Self::group_type, y: Self::group_type) -> Self::group_type {
-        Self::prod(x, Self::inv(y))
-    }
-}
+//     fn div(x: Self::group_type, y: Self::group_type) -> Self::group_type {
+//         Self::prod(x, Self::inv(y))
+//     }
+// }
 
 ////////////////////////
 // Impl for Secp256k1 //
